aneris/aneris_lang/state_interp/state_interp_free_ips_coh.v
@@ -20,36 +20,34 @@ Section state_interpretation.
   (** free_ips_coh *)
   Lemma free_ips_coh_init ip ips σ :
     ip ∉ ips →
-    dom (state_ports_in_use σ) = ips →
-    (∀ ip, ip ∈ ips → state_ports_in_use σ !! ip = Some ∅) →
     state_heaps σ = {[ip:=∅]} →
     state_sockets σ = {[ip:=∅]} →
     state_ms σ = ∅ →
     free_ips_auth ips ∗ free_ports_auth ∅ -∗ free_ips_coh σ.
   Proof.
-    iIntros (??? Hste Hsce ?) "[HipsCtx HPiu]".
+    iIntros (? Hste Hsce ?) "[HipsCtx HPiu]".
     iExists _, _; iFrame.
     rewrite Hste Hsce.
     iPureIntro.
-    do 2 (split; [set_solver|]).
-    split; [|set_solver].
-    intros ip' ?.
+    do 2 (split; try set_solver).
+    intros ip' ?. 
     assert (ip ≠ ip') by set_solver.
     rewrite !lookup_insert_ne //.
   Qed.
 
-  Lemma free_ips_coh_free_ports_valid σ a :
+  Lemma free_ips_coh_free_ports_valid σ a Sn :
+    state_sockets σ !! ip_of_address a = Some Sn → 
     free_ips_coh σ -∗
     free_ports (ip_of_address a) {[port_of_address a]} -∗
-    ∃ ps, ⌜state_ports_in_use σ !! ip_of_address a = Some ps ∧
-          port_of_address a ∉ ps⌝.
+    ⌜port_not_in_use (port_of_address a) Sn⌝.
   Proof.
-    iDestruct 1 as (Fip Piu (Hdsj & HFip & HFip2 & HPiu)) "[HfCtx HpCtx]".
-    iIntros "Hp".
+    iDestruct 1 as (Fip Piu (Hdsj & HFip)) "[HfCtx HpCtx]". iIntros "Hp". 
     iDestruct (free_ports_included with "HpCtx Hp") as (?) "[%Hlookup %]".
-    destruct (HPiu _ _ Hlookup) as (?&?&?).
-    iExists _. iPureIntro. split; [done|set_solver].
-  Qed.
+    unfold port_not_in_use. iPureIntro. intros sh skt sa r Hsh Hsa.
+    destruct HFip as [? HFip].
+    specialize (HFip (ip_of_address a) (ports') Hlookup Sn sh skt r sa H Hsh Hsa).
+    set_solver.
+  Qed.  
 
   Lemma free_ips_coh_alloc_node σ ip ports :
     free_ips_coh σ -∗
@@ -58,18 +56,19 @@ Section state_interpretation.
                     <| state_sockets := <[ip:=∅]> (state_sockets σ) |>) ∗
     free_ports ip ports.
   Proof.
-    iDestruct 1 as (Fip Piu (Hdsj & HFip & HFip2 & HPiu)) "[HfCtx HpCtx]".
+    iDestruct 1 as (Fip Piu (Hdsj & HFip)) "[HfCtx HpCtx]".
     iIntros "Hfip".
     iDestruct (free_ip_included with "HfCtx Hfip") as %Hin.
     iMod (free_ip_dealloc with "HfCtx Hfip") as "HfCtx".
     iMod (free_ports_alloc _ ip ports with "HpCtx") as "[HpCtx Hports]";
       [set_solver|].
     iModIntro. iFrame. iExists _, _. simpl. iFrame. iPureIntro.
-    split; [set_solver|]. split; [set_solver|]. split.
+    split; [set_solver|]. split.
     { intros. rewrite !lookup_insert_ne //; set_solver. }
-    intros ip' ??.
-    destruct (decide (ip = ip')); simplify_map_eq; [|eauto].
-    eexists; split; eauto. set_solver.
+    intros ip' ??????????.
+    destruct (decide (ip = ip')).
+    - subst. simpl_map. naive_solver.
+    - simplify_map_eq. eapply HFip; eauto.
   Qed.
 
   Lemma free_ips_coh_update_heap σ ip h h' :
@@ -78,83 +77,114 @@ Section state_interpretation.
     free_ips_coh (σ <| state_heaps := <[ip:=h']> (state_heaps σ) |>).
   Proof.
     iIntros (?).
-    iDestruct 1 as (Fip Piu (Hdsj & HFip & HFip2 & HPiu)) "[HfCtx HpCtx]".
+    iDestruct 1 as (Fip Piu (Hdsj & HFip)) "[HfCtx HpCtx]".
     iExists _, _. simpl. iFrame. iPureIntro.
-    do 3 (split; auto).
+    split; auto. split; try apply HFip.
     intros ip' ?.
     split; [|set_solver].
     destruct (decide (ip = ip')); simplify_map_eq; [set_solver|].
-    by apply HFip2.
+    by apply HFip.
   Qed.
 
-  Lemma free_ips_coh_alloc_socket σ ip Sn sh sock :
+  (* !!! gør den her pænere *)
+  Lemma free_ips_coh_alloc_socket σ ip Sn sh s:
     let σ' :=
-        σ <| state_sockets := <[ip:=<[sh:=sock]> Sn]> (state_sockets σ) |> in
+        σ <| state_sockets := <[ip:=<[sh:=(s, [])]> Sn]> (state_sockets σ) |> in
+    saddress s = None →    
     state_sockets σ !! ip = Some Sn →
     Sn !! sh = None →
     free_ips_coh σ -∗ free_ips_coh σ'.
   Proof.
-    iIntros (???).
-    iDestruct 1 as (Fip Piu (Hdsj & HFip & HFip2 & HPiu)) "[HfCtx HpCtx]".
+    iIntros (????).
+    iDestruct 1 as (Fip Piu (Hdsj & HFip)) "[HfCtx HpCtx]".
     iExists _, _. simpl. iFrame. iPureIntro.
-    do 3 (split; auto).
-    intros ip' ?.
-    split; [by eapply HFip2|].
+    split; auto. split.
+    - intros ip' ?.
+    split; [by eapply HFip|].
     destruct (decide (ip = ip')); simplify_map_eq; [set_solver|].
-    by apply HFip2.
+    by apply HFip.
+    - intros ip' ??????????.
+      destruct (decide (ip = ip')).
+      -- subst. simpl_map. inversion H3. subst.
+        destruct (decide (sh = sh0)).
+        + subst. apply (lookup_insert_rev Sn sh0 
+        (s, []) (skt, r)) in H4. 
+        inversion H4. rewrite -H7 in H5. set_solver. 
+        + apply (lookup_insert_ne Sn sh sh0 (s, [])) in n. 
+        rewrite n in H4. destruct HFip as [? HFip].
+        eapply HFip; eauto. 
+      -- simplify_map_eq. eapply HFip; eauto.
   Qed.
 
-  Lemma free_ips_coh_dealloc σ1 a sh skt Sn ps :
+  (* !!! gør den her pænere *)
+  Lemma free_ips_coh_dealloc σ1 a sh skt Sn :
     let ip := ip_of_address a in
     let S' := <[ip := <[sh:=(skt<| saddress := Some a |>, [])]> Sn]>
               (state_sockets σ1) in
-    let P' := <[ip := {[port_of_address a]} ∪ ps]> (state_ports_in_use σ1) in
-    let σ2 := σ1 <| state_sockets := S' |> <| state_ports_in_use := P' |> in
+    let σ2 := σ1 <| state_sockets := S' |>  in
     state_sockets σ1 !! ip = Some Sn →
-    state_ports_in_use σ1 !! ip = Some ps →
     free_ips_coh σ1 -∗
     free_ports (ip_of_address a) {[port_of_address a]} ==∗
     free_ips_coh σ2.
   Proof.
     rewrite /free_ips_coh /=.
-    iDestruct 1 as (Fip Piu (Hdsj & HFip & HFip2 & HPiu)) "[HfCtx HpCtx]".
+    iDestruct 1 as (Fip Piu (Hdsj & HFip)) "[HfCtx HpCtx]".
     iIntros "Hp".
     iMod (free_ports_dealloc with "HpCtx Hp")
       as (ps' [Hps' Hin%elem_of_subseteq_singleton]) "HpCtx".
     iModIntro. iExists _, _; iFrame. iPureIntro.
-    split; [set_solver|].
-    split.
-    { intros ip ?.
-      destruct (decide (ip = ip_of_address a)); simplify_eq; [set_solver|].
-      rewrite lookup_insert_ne //. by apply HFip. }
-    split.
-    { intros ip ?. split; [set_solver|].
-      destruct (decide (ip = ip_of_address a)); simplify_eq; [set_solver|].
-      rewrite lookup_insert_ne //. by apply HFip2. }
-    intros ip ??.
-    destruct (decide (ip = ip_of_address a)); simplify_map_eq.
-    - destruct (HPiu _ _ Hps') as [Q [Ha HQ]]. simplify_map_eq.
-      eexists. split; [done|]. set_solver.
-    - rewrite lookup_insert_ne //. set_solver.
-  Qed.
+    split; [set_solver|]. split.
+    - intros ip ?.
+    destruct (decide (ip = ip_of_address a)); simplify_eq; [set_solver|].
+    rewrite lookup_insert_ne //. by apply HFip.
+    - destruct HFip as [? HFip]. intros ip ps ?????????.
+      destruct (decide ((ip_of_address a) = ip)).
+      -- subst. specialize (HFip (ip_of_address a)).
+      simplify_map_eq. 
+      specialize (HFip ps' Hps'). 
+      specialize (HFip Sn sh0 skt0 r sa). 
+      specialize (HFip H).
+      destruct (decide (sh = sh0)).
+        + subst. apply (lookup_insert_rev Sn sh0 
+        ({| saddress := Some a; sblock := sblock skt |}, []) (skt0, r))  in H3.
+        inversion H3. subst. simpl in H4. inversion H4. set_solver. 
+        + apply (lookup_insert_ne Sn sh sh0 
+        ({| saddress := Some a; sblock := sblock skt |}, []))  in n. 
+        rewrite n in H3.
+        specialize (HFip H3 H4). set_solver.
+      -- simplify_map_eq. eapply HFip; eauto.
+  Qed. 
 
-  Lemma free_ips_coh_update_msg sh a skt Sn r' σ1 :
+  (* !!! gør den her pænere *)
+  Lemma free_ips_coh_update_msg sh a skt Sn r m σ1 :
     let ip := ip_of_address a in
-    let S' := <[ip := <[sh:=(skt, r')]> Sn]> (state_sockets σ1) in
+    let S' := <[ip := <[sh:=(skt, r)]> Sn]> (state_sockets σ1) in
     let σ2 := σ1 <| state_sockets := S' |> in
+    Sn !! sh = Some (skt, r ++ [m]) →
     state_sockets σ1 !! ip_of_address a = Some Sn →
     free_ips_coh σ1 -∗ free_ips_coh σ2.
   Proof.
     rewrite /free_ips_coh /=.
-    iDestruct 1 as (Fip Piu (Hdsj & HFip & HFip2 & HPiu)) "[HfCtx HpCtx]".
-    iExists _, _. simpl. iFrame. iPureIntro.
-    do 2 (split; [auto|]).
-    split; [|done].
-    intros ip ?. split; [set_solver|].
-    destruct (decide (ip = ip_of_address a)); simplify_map_eq; [set_solver|].
-    by apply HFip2.
+    iDestruct 1 as (Fip Piu (Hdsj & HFip)) "[HfCtx HpCtx]".
+    iExists _, _. iFrame. iPureIntro.
+      split; [auto|]. split.
+      - intros ip ?. split; [set_solver|].
+        destruct (decide (ip = ip_of_address a)); simplify_map_eq; [set_solver|].
+        by apply HFip.
+      - intros ip ??????????. destruct HFip as [? HFip].
+        destruct (decide ((ip_of_address a) = ip)).
+        --- subst. simpl_map. inversion H2. subst.
+        destruct (decide (sh = sh0)).
+          + subst. apply (lookup_insert_rev Sn sh0 
+          (skt, r) (skt0, r0)) in H3. 
+          inversion H3. rewrite -H7 in H4.
+          eapply HFip; eauto. 
+          + apply (lookup_insert_ne Sn sh sh0 (skt, r))  in n. 
+          rewrite n in H3. eapply HFip; eauto.  
+        --- simplify_map_eq. eapply HFip; eauto.   
   Qed.
 
+  (* !!! gør den her pænere *)
   Lemma free_ips_coh_deliver_message σ M Sn Sn' ip sh skt a R m :
     m ∈ messages_to_receive_at a M →
     (state_sockets σ) !! ip = Some Sn →
@@ -165,21 +195,33 @@ Section state_interpretation.
     free_ips_coh
       {| state_heaps := state_heaps σ;
          state_sockets := <[ip:=Sn']> (state_sockets σ);
-         state_ports_in_use := state_ports_in_use σ;
          state_ms := state_ms σ |}.
   Proof.
     rewrite /free_ips_coh /=.
-    iDestruct 1 as (Fip Piu (Hdsj & HFip & HFip2 & HPiu)) "[HfCtx HpCtx]".
+    iDestruct 1 as (Fip Piu (Hdsj & HFip)) "[HfCtx HpCtx]".
     iExists _, _. simpl. iFrame. iPureIntro.
-    do 2 (split; [auto|]).
-    split; [|done].
-    intros ip' ?. split; [set_solver|].
-    ddeq ip ip'.
-    - naive_solver.
-    - destruct (decide (ip' = ip_of_address a)); simplify_map_eq; [set_solver|].
-      by apply HFip2.
-  Qed.
+    split; [auto|]. split.
+    - intros ip' ?.
+      ddeq ip ip'.
+      -- naive_solver.
+      -- destruct (decide (ip' = ip_of_address a)); simplify_map_eq; [set_solver|].
+        by apply HFip.
+    - intros ip' ??????????.
+      destruct (decide (ip = ip')).
+      -- subst. simpl_map. inversion H5. rewrite -H8 in H6.
+      destruct HFip as [? HFip].
+      specialize (HFip ip' ps H4). 
+      destruct (decide (sh = sh0)).
+      + subst. apply (lookup_insert_rev Sn sh0 
+      (skt, m :: R) (skt0, r)) in H6. inversion H6. rewrite -H9 in H7.
+      eapply HFip; eauto. 
+      + apply (lookup_insert_ne Sn sh sh0 
+      (skt, m :: R)) in n. rewrite n in H6.
+      eapply HFip; eauto.  
+      -- simplify_map_eq. eapply HFip; eauto.
+  Qed.      
 
+  (* !!! gør den her pænere *)
   Lemma free_ips_coh_update_sblock σ1 a Sn sh skt b r :
     let ip := ip_of_address a in
     let S := <[ip := <[sh:= (skt<| sblock := b|>, r)]> Sn]>(state_sockets σ1) in
@@ -189,25 +231,38 @@ Section state_interpretation.
     free_ips_coh σ1 ==∗ free_ips_coh σ2.
   Proof.
     iIntros (?).
-    iDestruct 1 as (Fip Piu (Hdsj & HFip & HFip2 & HPiu)) "[HfCtx HpCtx]".
+    iDestruct 1 as (Fip Piu (Hdsj & HFip)) "[HfCtx HpCtx]".
     iExists _, _. simpl. iFrame. iPureIntro.
-    do 3 (split; auto).
-    intros ip' Hip'.
+    split; auto. split.
+    - intros ip' Hip'.
     simplify_map_eq. subst S.
     ddeq ip ip'; set_solver.
+    - intros ip' ??????????.
+      destruct HFip as [? HFip].
+      specialize (HFip ip' ps H1).
+      unfold S in H2.
+      destruct (decide (ip = ip')).
+      -- subst. simpl_map. inversion H2. rewrite -H7 in H3.
+      destruct (decide (sh = sh0)).
+      + subst. apply (lookup_insert_rev Sn sh0 
+      ({| saddress := saddress skt; sblock := b |}, r) (skt0, r0)) in H3. 
+      inversion H3. rewrite -H7 in H4. simpl in H4.
+      eapply HFip; eauto. 
+      + apply (lookup_insert_ne Sn sh sh0 
+      ({| saddress := saddress skt; sblock := b |}, r)) in n. rewrite n in H3.
+      eapply HFip; eauto.  
+      -- simplify_map_eq. eapply HFip; eauto.
   Qed.
-
-  Lemma free_ips_coh_ms hps skts ports ms1 ms2 :
+      
+  Lemma free_ips_coh_ms hps skts ms1 ms2 :
     free_ips_coh {|
       state_heaps := hps;
       state_sockets := skts;
-      state_ports_in_use := ports;
       state_ms := ms1;
       |} -∗
     free_ips_coh {|
       state_heaps := hps;
       state_sockets := skts;
-      state_ports_in_use := ports;
       state_ms := ms2;
     |}.
   Proof. done. Qed.
