aneris/examples/ccddb/examples/message_passing/proof_adequacy.v
@@ -18,8 +18,6 @@ Definition init_state :=
   {|
     state_heaps := {[ "system" := ∅ ]};
     state_sockets := {[ "system" := ∅ ]};
-    state_ports_in_use :=
-      <["0.0.0.0" := ∅ ]> $ <["0.0.0.1" := ∅ ]> $ ∅;
     state_ms := ∅;
   |}.
 
@@ -61,9 +59,6 @@ Proof.
  eapply (@adequacy Σ dummy_model _ _ ips sa_dom ∅ ∅ ∅);
    try done; last first.
   { set_solver. }
-  { intros i. rewrite /ips !elem_of_union !elem_of_singleton.
-    intros [|]; subst; simpl; set_solver. }
-  { rewrite /ips /= !dom_insert_L dom_empty_L right_id_L //. }
   2: { apply dummy_model_finitary. }
   iIntros (Hdg) "".
   iPoseProof (main_spec sa_dom) as "Hmain".
